

Early +1

Amelhyang 2020 AST 322 1215293924 HW3

3/3 3.1.  $(\Delta S')^2 = -c^2(\Delta t')^2 + (\Delta x')^2 + (\Delta y')^2 + (\Delta z')^2$  ✓  
 $= -\gamma^2 \left[ c(t_1 - t_2) - \frac{v}{c}(x_1 - x_2) \right]^2 + \gamma^2 \left[ x_1 - x_2 - v(t_1 - t_2) \right]^2 + (y_1 - y_2)^2 + (z_1 - z_2)^2$  ✓  
 where  $\gamma = \frac{1}{\sqrt{1 - v^2/c^2}}$  ✓ (3.20 is correct below)

Then, ignoring the y and z terms for now,  
 $(\Delta S')^2 = -\frac{1}{1 - \frac{v^2}{c^2}} \left( c(t_1 - t_2) - \frac{v}{c}(x_1 - x_2) \right)^2$   
 $+ \frac{1}{1 - \frac{v^2}{c^2}} \left( x_1 - x_2 - v(t_1 - t_2) \right)^2$

Let  $x_1 - x_2 = \Delta x$  and  $t_1 - t_2 = \Delta t$ . The equation becomes  
 $(\Delta S')^2 = \frac{1}{1 - \frac{v^2}{c^2}} \left( c^2 \Delta t^2 + \frac{v^2}{c^2} \Delta x^2 - 2v \Delta t \Delta x \right) + \frac{1}{1 - \frac{v^2}{c^2}} \left( \Delta x^2 + v^2 \Delta t^2 - 2v \Delta x \Delta t \right)$   
 $= \frac{1}{1 - \frac{v^2}{c^2}} \left( \Delta x^2 + v^2 \Delta t^2 - c^2 \Delta t^2 - \frac{v^2}{c^2} \Delta x^2 \right)$   
 $= \frac{1}{1 - \frac{v^2}{c^2}} \Delta x^2 \left( 1 - \frac{v^2}{c^2} \right) - \frac{1}{1 - \frac{v^2}{c^2}} c^2 \Delta t^2 \left( 1 - \frac{v^2}{c^2} \right)$   
 $= -c^2 \Delta t^2 + \Delta x^2$

$= -c^2(t_1 - t_2)^2 + (x_1 - x_2)^2 + (y_1 - y_2)^2 + (z_1 - z_2)^2 = (\Delta S)^2$  ✓  
 so that  $(\Delta S')^2 = (\Delta S)^2$  and the 3.21 is shown from 3.20.

In showing 3.20,  $-c^2(\Delta t')^2 + (\Delta x')^2 + (\Delta y')^2 + (\Delta z')^2$   
 $= -\gamma^2 \left[ c(t_1 - t_2) - \frac{v}{c}(x_1 - x_2) \right]^2 + \gamma^2 \left[ x_1 - x_2 - v(t_1 - t_2) \right]^2 + (y_1 - y_2)^2 + (z_1 - z_2)^2$

Note that  $x' = \gamma(x - vt)$ ,  $y' = y$ ,  $z' = z$ , and  $t' = \gamma(t - vx/c^2)$  (3.11) so that

$(\Delta t')^2 = \gamma^2 [x_1 - x_2 - v(t_1 - t_2)]^2 + (y_1 - y_2)^2 + (z_1 - z_2)^2$  ✓  
 (3.15) and

$$\Delta t' = t_1' - t_2' = \gamma \left[ (t_1 - t_2) - \frac{v}{c^2} (x_1 - x_2) \right] \quad (3.16) \checkmark$$

Substituting these values:

$$\begin{aligned} (\Delta s')^2 &= -c^2 (\Delta t')^2 + (\Delta L')^2 = -c^2 (t_1' - t_2')^2 + (x_1' - x_2')^2 \\ &+ (y_1' - y_2')^2 + (z_1' - z_2')^2 \\ &= -\gamma^2 \left[ c^2 \left( (t_1 - t_2) - \frac{v}{c^2} (x_1 - x_2) \right)^2 + \gamma^2 \left[ (x_1 - x_2 - v(t_1 - t_2))^2 \right. \right. \\ &\left. \left. + (y_1 - y_2)^2 + (z_1 - z_2)^2 \right] \right] \checkmark \end{aligned}$$

and 3.20 is shown, which 3.21 follows as shown before.

2/2 3.2. For a box length  $2m$ , the time light takes to travel is  $\Delta t = \frac{d}{v} = \frac{d}{c} = \frac{2m}{3 \times 10^8 \text{ m/s}}$

With  $a = -9.8 \text{ m/s}^2$ , during  $\Delta t$  the light travels downwards

$$\Delta x = \frac{1}{2} a t^2 = \frac{1}{2} g \frac{d^2}{c^2} = \frac{1}{2} (9.81) \left( \frac{2}{3 \times 10^8} \right)^2 \approx 2 \times 10^{-16} \text{ m} \checkmark$$

and shown

5/5 3.3. If  $dl^2 = dr^2 + S_K(r)^2 d\Omega^2$ , show that equals  $dl^2 = \frac{dr^2}{1 - Kx^2/R^2} + \bar{x}^2 d\Omega^2$  where  $\bar{x}^2 = S_K(r)$

$$\text{and } S_K(r) = \begin{cases} R \sin(r/R) & (K=+1) \\ r & (K=0) \\ R \sinh(r/R) & (K=-1) \end{cases}$$

For  $K=1$ , using the second equation:

$$d\bar{x} = \cos\left(\frac{r}{R}\right) dr \rightarrow dl^2 = \frac{\cos^2\left(\frac{r}{R}\right) dr^2}{1 - \sin^2\left(\frac{r}{R}\right)} + \bar{x}^2 d\Omega^2 = \frac{\cos^2\left(\frac{r}{R}\right) dr^2}{\cos^2\left(\frac{r}{R}\right)} + \bar{x}^2 d\Omega^2$$

$$= dr^2 + \bar{x}^2 d\Omega^2 = dr^2 + S_K(r)^2 d\Omega^2 \checkmark \text{ and the two equations are equal}$$

$$\text{For } K=0, dl^2 = \frac{dr^2}{1 - 0 \cdot x^2/R^2} + \bar{x}^2 d\Omega^2 = dr^2 + S_K(r)^2 d\Omega^2 \checkmark$$

and are equal

$$\text{For } K=-1, d\bar{x} = \cosh\left(\frac{r}{R}\right) dr \rightarrow dl^2 = \frac{\cosh^2\left(\frac{r}{R}\right) dr^2}{1 + \sinh^2\left(\frac{r}{R}\right)} + \bar{x}^2 d\Omega^2$$

$$= \frac{\cosh^2\left(\frac{r}{R}\right)}{\cosh^2\left(\frac{r}{R}\right)} dr^2 + \bar{x}^2 d\Omega^2 = dr^2 + S_K(r)^2 d\Omega^2 \checkmark \text{ and are equal}$$